MemoryMappedExtCalls with just read_step and write_step,
used to define bedrock2 ext_spec as well as risc-v nonmem_load_store

bedrock2/src/bedrock2/memory_mapped_ext_spec.v
@@ -18,30 +18,14 @@ Proof.
 Qed.
 
 Class MemoryMappedExtCalls{width: Z}{BW: Bitwidth width}
-                          {word: word.word width} {mem: map.map word Byte.byte} := {
-  mmio_read_step:
+                          {word: word.word width}{mem: map.map word Byte.byte} := {
+  read_step:
     nat -> (* how many bytes to read *)
     trace -> (* trace of events that happened so far *)
     word -> (* address to be read *)
     (word -> mem -> Prop) -> (* postcondition on returned value and memory *)
     Prop;
-  mmio_write_step:
-    nat -> (* how many bytes to write *)
-    trace -> (* trace of events that happened so far *)
-    word -> (* address to be written *)
-    word -> (* value to be written *)
-    mem -> (* memory whose ownership is passed to the external world *)
-    Prop;
-  (* same signatures for accessing shared memory, i.e. memory that has been passed
-     to the external world, but might still be accessible under some conditions,
-     and can change each time it is looked at *)
-  shared_mem_read_step:
-    nat -> (* how many bytes to read *)
-    trace -> (* trace of events that happened so far *)
-    word -> (* address to be read *)
-    (word -> mem -> Prop) -> (* postcondition on returned value and memory *)
-    Prop;
-  shared_mem_write_step:
+  write_step:
     nat -> (* how many bytes to write *)
     trace -> (* trace of events that happened so far *)
     word -> (* address to be written *)
@@ -55,50 +39,32 @@ Section WithMem.
           {word: word.word width} {mem: map.map word Byte.byte}.
   Context {word_ok: word.ok word}.
 
-  Inductive ext_spec{mmio_ext_calls: MemoryMappedExtCalls}: ExtSpec :=
-  | ext_spec_mmio_read: forall t addr n post,
-      mmio_read_step n t addr (fun v mRcv => post mRcv [v]) ->
-      ext_spec t map.empty ("MMIO_READ" ++ String.of_nat (n * 8)) [addr] post
-  | ext_spec_mmio_write: forall t addr n mGive v post,
-      mmio_write_step n t addr v mGive ->
-      post map.empty nil ->
-      ext_spec t mGive ("MMIO_WRITE" ++ String.of_nat (n * 8)) [addr; v] post
-  | ext_spec_shared_mem_read: forall t addr n post,
-      shared_mem_read_step n t addr (fun v mRcv => post mRcv [v]) ->
-      ext_spec t map.empty ("SHARED_MEM_READ" ++ String.of_nat (n * 8)) [addr] post
-  | ext_spec_shared_mem_write: forall t addr n mGive v post,
-      shared_mem_write_step n t addr v mGive ->
-      post map.empty nil ->
-      ext_spec t mGive ("SHARED_MEM_WRITE" ++ String.of_nat (n * 8)) [addr; v] post.
+  Definition ext_spec{mmio_ext_calls: MemoryMappedExtCalls}: ExtSpec :=
+    fun (t: trace) (mGive: mem) (action: string) (args: list word)
+        (post: mem -> list word -> Prop) =>
+      exists n, (n = 1 \/ n = 2 \/ n = 4 \/ (n = 8 /\ width = 64%Z))%nat /\
+      ((action = "memory_mapped_extcall_read" ++ String.of_nat (n * 8) /\
+        exists addr, args = [addr] /\ mGive = map.empty /\
+                     read_step n t addr (fun v mRcv => post mRcv [v])) \/
+       (action = "memory_mapped_extcall_write" ++ String.of_nat (n * 8) /\
+        exists addr val, args = [addr; val] /\
+                         write_step n t addr val mGive /\
+                         post map.empty nil)).
 
-  Class MemoryMappedExtCallsOk(mmio_ext_calls: MemoryMappedExtCalls): Prop := {
-    weaken_mmio_read_step: forall t addr n post1 post2,
-      mmio_read_step n t addr post1 ->
+  Class MemoryMappedExtCallsOk(ext_calls: MemoryMappedExtCalls): Prop := {
+    weaken_read_step: forall t addr n post1 post2,
+      read_step n t addr post1 ->
       (forall v mRcv, post1 v mRcv -> post2 v mRcv) ->
-      mmio_read_step n t addr post2;
-    intersect_mmio_read_step: forall t addr n post1 post2,
-      mmio_read_step n t addr post1 ->
-      mmio_read_step n t addr post2 ->
-      mmio_read_step n t addr (fun v mRcv => post1 v mRcv /\ post2 v mRcv);
-    mmio_write_step_unique_mGive: forall m t n mKeep1 mKeep2 mGive1 mGive2 addr val,
+      read_step n t addr post2;
+    intersect_read_step: forall t addr n post1 post2,
+      read_step n t addr post1 ->
+      read_step n t addr post2 ->
+      read_step n t addr (fun v mRcv => post1 v mRcv /\ post2 v mRcv);
+    write_step_unique_mGive: forall m t n mKeep1 mKeep2 mGive1 mGive2 addr val,
       map.split m mKeep1 mGive1 ->
       map.split m mKeep2 mGive2 ->
-      mmio_write_step n t addr val mGive1 ->
-      mmio_write_step n t addr val mGive2 ->
-      mGive1 = mGive2;
-    weaken_shared_mem_read_step: forall t addr n post1 post2,
-      shared_mem_read_step n t addr post1 ->
-      (forall v mRcv, post1 v mRcv -> post2 v mRcv) ->
-      shared_mem_read_step n t addr post2;
-    intersect_shared_mem_read_step: forall t addr n post1 post2,
-      shared_mem_read_step n t addr post1 ->
-      shared_mem_read_step n t addr post2 ->
-      shared_mem_read_step n t addr (fun v mRcv => post1 v mRcv /\ post2 v mRcv);
-    shared_mem_write_step_unique_mGive: forall m t n mKeep1 mKeep2 mGive1 mGive2 addr val,
-      map.split m mKeep1 mGive1 ->
-      map.split m mKeep2 mGive2 ->
-      shared_mem_write_step n t addr val mGive1 ->
-      shared_mem_write_step n t addr val mGive2 ->
+      write_step n t addr val mGive1 ->
+      write_step n t addr val mGive2 ->
       mGive1 = mGive2;
   }.
 
@@ -109,8 +75,7 @@ Section WithMem.
       ext_spec t mGive a args post1 ->
       ext_spec t mGive a args post2.
   Proof.
-    intros; inversion H0; subst; clear H0;
-      constructor; eauto using weaken_mmio_read_step, weaken_shared_mem_read_step.
+    unfold ext_spec; intros; fwd; destruct H0p1; fwd; eauto 10 using weaken_read_step.
   Qed.
 
   Instance ext_spec_ok(mmio_ext_calls: MemoryMappedExtCalls)
@@ -118,15 +83,17 @@ Section WithMem.
   Proof.
     constructor.
     - (* mGive unique *)
-      intros. inversion H1; subst; clear H1; inversion H2; subst; clear H2;
-        fwd; eauto using mmio_write_step_unique_mGive, shared_mem_write_step_unique_mGive.
+      unfold ext_spec. intros. fwd. destruct H1p1; destruct H2p1; fwd; try congruence.
+      inversion H1p1. fwd. eauto using write_step_unique_mGive.
     - (* weaken *)
       unfold Morphisms.Proper, Morphisms.respectful, Morphisms.pointwise_relation,
         Basics.impl. eapply weaken_ext_spec.
     - (* intersect *)
-      intros. inversion H; subst; clear H; inversion H0; subst; clear H0; fwd;
-        constructor;
-        eauto using intersect_mmio_read_step, intersect_shared_mem_read_step.
+      unfold ext_spec. intros. fwd. destruct Hp1; destruct H0p1; fwd;
+        match goal with
+        | H: _ ++ _ = _ ++ _ |- _ => inversion H; clear H
+        end;
+        fwd; eauto 10 using intersect_read_step.
   Qed.
 
 End WithMem.
